start de Bruijn version

theories/Semantics.v
@@ -1,35 +1,29 @@
 Require Import ssreflect.
-From Malfunction Require Import Malfunction Interpreter.
 
 Require Import ZArith Array.PArray List String Floats Lia.
 Import ListNotations.
+
+Require Malfunction.Malfunction Malfunction.SemanticsSpec.
+Module N := Malfunction.Malfunction.
+Module Spec := Malfunction.SemanticsSpec.
+Import N.
+
+From Malfunction Require Import Ast.
 
 Set Default Goal Selector "!".
 
 Inductive value :=
 | Block of int * list value
 | Vec of vector_type * list value
-| Func of Ident.t * @Ident.Map.t value * t
+| Func of Ident.t * (list (Ident.t * value)) * t
 | value_Int of inttype * Z
 | Float of float
 | Thunk of value
 | fail of string
 .
 
-Fixpoint vtrans (s : value) : Interpreter.value :=
-  match s with
-  | Block (tag, vals) => Interpreter.Block (tag, Array_of_list (Interpreter.fail "") (map vtrans vals))
-  | Vec (ty, vals) => Interpreter.Vec (ty, Array_of_list (Interpreter.fail "") (map vtrans vals))
-  | Func (x, locals, e) => Interpreter.Func (fun v => interpret (Ident.Map.add x v (fun x => vtrans (locals x))) e)
-  | value_Int (ty, i) => Interpreter.value_Int (ty, i)
-  | Float f => Interpreter.Float f
-  | Thunk v => Interpreter.Thunk (vtrans v)
-  | fail x => Interpreter.fail x
-  end.
-
 Definition int_to_nat (i : int) : nat :=
   Z.to_nat (Int63.to_Z i).
-
 
 Definition cond scr case : bool := 
   (match case, scr with
@@ -50,20 +44,24 @@ Fixpoint find_match scr x : option t := match x with
 Definition Mklambda binders e :=
   match binders with [] => e | _ => Mlambda (binders, e) end.
 
-Fixpoint add_recs' (locals : Ident.Map.t) allrecs recs  :=
+Definition scons {A} x (f : nat -> A) := 
+  fun n =>
+    match n with 
+    | 0 => x
+    | S n => f n
+    end.
+
+Fixpoint add_recs' (locals : list (Ident.t * value)) (allrecs recs : list (Ident.t * t)) : option (list (Ident.t * value)) :=
   match recs with
   | [] => Some locals
   | (x, Mlambda (y :: more, e)) :: recs =>  
-    match add_recs' locals allrecs recs with
-    | Some locals => Some (Ident.Map.add x (Func (y, locals, Mlet ([Recursive allrecs], Mklambda more e))) locals)
-    | None => None
-    end
+     add_recs' (cons (x, Func (y, locals, Mlet ([Recursive allrecs], Mklambda more e))) locals) allrecs recs
   | _ => None
   end.
 Definition add_recs locals recs := add_recs' locals recs recs.
 
 Unset Elimination Schemes.           
-Inductive eval (locals : @Ident.Map.t value) : t -> value -> Prop :=
+Inductive eval (locals : list (Ident.t * value)) : t -> value -> Prop :=
 | eval_lambda_sing x e :
   eval locals (Mlambda ([x], e)) (Func (x, locals, e))
 | eval_lambda x ids e :
@@ -71,13 +69,14 @@ Inductive eval (locals : @Ident.Map.t value) : t -> value -> Prop :=
   eval locals (Mlambda (x :: ids, e)) (Func (x, locals, Mlambda (ids, e)))
 | eval_app_sing x locals' e e2 v2 e1 v :
   eval locals e1 (Func (x, locals', e)) -> eval locals e2 v2 ->
-  eval (Ident.Map.add x v2 locals') e v ->
+  eval (cons (x, v2) locals') e v ->
   eval locals (Mapply (e1, [e2])) v
 | eval_app e2 e1 v es :
   eval locals (Mapply (Mapply (e1, [e2]), es)) v ->
   eval locals (Mapply (e1, e2 :: es)) v
-| eval_var id :
-  eval locals (Mvar id) (Ident.Map.find id locals)
+| eval_var n x v :
+  nth_error locals n = Some (x, v) ->
+  eval locals (Mvar n) v
 | eval_let_body e v : 
   eval locals e v -> eval locals (Mlet ([], e)) v
 | eval_let_unnamed e1 v1 lts e2 v :
@@ -86,7 +85,7 @@ Inductive eval (locals : @Ident.Map.t value) : t -> value -> Prop :=
   eval locals (Mlet (Unnamed e1 :: lts, e2)) v 
 | eval_let_named x e1 v1 lts e2 v :
   eval locals e1 v1 ->
-  eval (Ident.Map.add x v1 locals) (Mlet (lts, e2)) v ->
+  eval (cons (x, v1) locals) (Mlet (lts, e2)) v ->
   eval locals (Mlet (Named (x,e1) :: lts, e2)) v 
 | eval_let_rec recs newlocals lts e2 v :
   add_recs locals recs = Some newlocals ->
@@ -107,64 +106,65 @@ Inductive eval (locals : @Ident.Map.t value) : t -> value -> Prop :=
   eval locals (Mfield (idx, b)) (nth (int_to_nat idx) vals (fail "")).
 
 Lemma eval_ind :
-forall P : Ident.Map.t -> t -> value -> Prop,
-(forall (locals : Ident.Map.t) (x : Ident.t) (e : t),
+forall P : (list (Ident.t * value)) -> t -> value -> Prop,
+(forall (locals : (list (Ident.t * value))) (x : Ident.t) (e : t),
  P locals (Mlambda ([x], e)) (Func (x, locals, e))) ->
-(forall (locals : Ident.Map.t) (x : Ident.t) (ids : list Ident.t) (e : t),
+(forall (locals : (list (Ident.t * value))) (x : Ident.t) (ids : list Ident.t) (e : t),
  Datatypes.length ids > 0 ->
  P locals (Mlambda (x :: ids, e)) (Func (x, locals, Mlambda (ids, e)))) ->
-(forall (locals : Ident.Map.t) (x : Ident.t) (locals' : Ident.Map.t) 
+(forall (locals : (list (Ident.t * value))) (x : Ident.t) (locals' : (list (Ident.t * value))) 
    (e e2 : t) (v2 : value) (e1 : t) (v : value),
  eval locals e1 (Func (x, locals', e)) ->
  P locals e1 (Func (x, locals', e)) ->
  eval locals e2 v2 ->
  P locals e2 v2 ->
- eval (Ident.Map.add x v2 locals') e v ->
- P (Ident.Map.add x v2 locals') e v -> P locals (Mapply (e1, [e2])) v) ->
-(forall (locals : Ident.Map.t) (e2 e1 : t) (v : value) (es : list t),
+ eval (cons (x, v2) locals') e v ->
+ P (cons (x, v2) locals') e v -> P locals (Mapply (e1, [e2])) v) ->
+(forall (locals : (list (Ident.t * value))) (e2 e1 : t) (v : value) (es : list t),
  eval locals (Mapply (Mapply (e1, [e2]), es)) v ->
  P locals (Mapply (Mapply (e1, [e2]), es)) v -> P locals (Mapply (e1, e2 :: es)) v) ->
-(forall (locals : Ident.Map.t) (id : Ident.t),
- P locals (Mvar id) (Ident.Map.find id locals)) ->
- (forall (locals : Ident.Map.t) (e : t) (v : value),
+(forall (locals : (list (Ident.t * value))) (n : nat) x v ,
+  nth_error locals n = Some (x, v) ->
+ P locals (Mvar n) v) ->
+ (forall (locals : (list (Ident.t * value))) (e : t) (v : value),
  eval locals e v -> P locals e v -> P locals (Mlet ([], e)) v) ->
-(forall (locals : Ident.Map.t) (e1 : t) (v1 : value) 
+(forall (locals : (list (Ident.t * value))) (e1 : t) (v1 : value) 
    (lts : list binding) (e2 : t) (v : value),
  eval locals e1 v1 ->
  P locals e1 v1 ->
  eval locals (Mlet (lts, e2)) v ->
  P locals (Mlet (lts, e2)) v -> P locals (Mlet (Unnamed e1 :: lts, e2)) v) ->
-(forall (locals : Ident.Map.t) (x : Ident.t) (e1 : t) 
+(forall (locals : (list (Ident.t * value))) (x : Ident.t) (e1 : t) 
    (v1 : value) (lts : list binding) (e2 : t) (v : value),
  eval locals e1 v1 ->
  P locals e1 v1 ->
- eval (Ident.Map.add x v1 locals) (Mlet (lts, e2)) v ->
- P (Ident.Map.add x v1 locals) (Mlet (lts, e2)) v ->
+ eval (cons (x, v1) locals) (Mlet (lts, e2)) v ->
+ P (cons (x, v1) locals) (Mlet (lts, e2)) v ->
  P locals (Mlet (Named (x, e1) :: lts, e2)) v) ->
-(forall (locals : Ident.Map.t) (recs : list (Ident.t * t))
-   (newlocals : Ident.Map.t) (lts : list binding) 
+(forall (locals : (list (Ident.t * value))) (recs : list (Ident.t * t))
+   (newlocals : (list (Ident.t * value))) (lts : list binding) 
    (e2 : t) (v : value),
  add_recs locals recs = Some newlocals ->
  eval newlocals (Mlet (lts, e2)) v ->
  P newlocals (Mlet (lts, e2)) v ->
  P locals (Mlet (Recursive recs :: lts, e2)) v) ->
-(forall (locals : Ident.Map.t) (scr : t) (cases : list (list case * t))
+(forall (locals : (list (Ident.t * value))) (scr : t) (cases : list (list case * t))
    (v v' : value) (e : t),
  eval locals scr v' ->
  P locals scr v' ->
  find_match v' cases = Some e ->
  eval locals e v -> P locals e v -> P locals (Mswitch (scr, cases)) v) ->
-(forall (locals : Ident.Map.t) (tag : int) (es : list t) (vals : list value),
+(forall (locals : (list (Ident.t * value))) (tag : int) (es : list t) (vals : list value),
     Forall2 (eval locals) es vals ->
     Forall2 (P locals) es vals ->
     P locals (Mblock (tag, es)) (Block (tag, vals))) ->
-(forall (locals : Ident.Map.t) (idx : int) (b : t) (vals : list value) (tag : int),
+(forall (locals : (list (Ident.t * value))) (idx : int) (b : t) (vals : list value) (tag : int),
  eval locals b (Block (tag, vals)) ->
  P locals b (Block (tag, vals)) ->
  Datatypes.length vals < Z.to_nat Int63.wB ->
  Datatypes.length vals <= int_to_nat max_length ->
  P locals (Mfield (idx, b)) (nth (int_to_nat idx) vals (fail ""))) ->
-forall (locals : Ident.Map.t) (t : t) (v : value), eval locals t v -> P locals t v.
+forall (locals : (list (Ident.t * value))) (t : t) (v : value), eval locals t v -> P locals t v.
 Proof.
   intros P H_lambda_sing H_lambda H_app_sing H_app H_var H_let_body H_let_unnamed H_let_named 
         H_let_rec H_switch H_block H_field.
@@ -177,292 +177,280 @@ Proof.
 Qed.
 Set Elimination Schemes.
 
-Axiom funext : forall A B, forall f g : A -> B, (forall x, f x = g x) -> f = g.
+Fixpoint names (x : t) {struct x} : list (Ident.t) :=
+  match x with
+  | Mvar v => []
+  | Mlambda (xs, e) =>
+      xs ++ names e
+  | Mapply (f, vs) =>
+      names f ++ flat_map names vs
+  | Mlet (bindings, body) =>
+      flat_map namesb bindings ++ names body
+  | Mswitch (scr, cases) =>
+      names scr ++ flat_map (fun '(_, e) => names e) cases
+  | Mnumop1 (op, _, e) =>
+      names e
+  | Mnumop2 (op, _, e1, e2) =>
+      names e1 ++ names e2
+  | Mconvert (_, _, e) =>
+      names e
+  | Mvecnew (ty, len, def) =>
+      names len ++ names def
+  | Mvecget (ty, vec, idx) =>
+      names vec ++ names idx 
+  | Mvecset (ty, vec, idx, e) => names vec ++ names idx ++ names e
+  | Mveclen (ty, vec) =>
+      names vec
+  | Mblock (idx, es) =>
+      flat_map names es
+  | Mfield (idx, b) =>
+      names b
+  | Mlazy e => names e
+  | Mforce e => names e
+  | _ => []
+  end
+with namesb (b : binding) : list (Ident.t) :=
+       match b with
+       | Unnamed e => names e
+       | Named (x, e) => x :: names e
+       | Recursive l => flat_map (fun '(x,e) => names e) l
+       end.
 
-Definition int_of_nat n := Int63.of_Z (Z.of_nat n).
+Definition bound_names  (b : binding) : list (Ident.t) :=
+  match b with
+  | Unnamed e => []
+  | Named (x, e) => [x]
+  | Recursive l => map (fun '(x,e) => x) l
+  end.
 
-Lemma int_of_to_nat i :
-  int_of_nat (int_to_nat i) = i.
+Fixpoint inb {A} (eqb : A -> A -> bool) (x : A) (l : list A) : bool :=
+  match l with
+  | [] => false
+  | y :: l => eqb x y || inb eqb x l
+  end.
+
+Definition disj : list Ident.t -> list Ident.t -> bool :=
+fun l1 l2 =>
+  forallb (fun x => negb (inb String.eqb x l2)) l1.
+
+Fixpoint wf (x : t) {struct x} : bool :=
+  match x with
+  | Mvar v => true
+  | Mlambda (xs, e) =>
+      disj (names e) xs && wf e
+  | Mapply (f, vs) =>
+     wf f && forallb wf vs
+  
+   | Mlet (bindings, body) =>
+      forallb wfb bindings && wf body && disj (flat_map bound_names bindings) (names body)
+  
+  | Mswitch (scr, cases) =>
+      wf scr && forallb (fun '(_, e) => wf e) cases
+  | Mnumop1 (op, _, e) =>
+      wf e
+  | Mnumop2 (op, _, e1, e2) =>
+      wf e1 && wf e2
+  | Mconvert (_, _, e) =>
+      wf e
+  | Mvecnew (ty, len, def) =>
+      wf len && wf def
+  | Mvecget (ty, vec, idx) =>
+      wf vec && wf idx 
+  | Mvecset (ty, vec, idx, e) => 
+      wf vec && wf idx && wf e
+  | Mveclen (ty, vec) =>
+      wf vec
+  | Mblock (idx, es) =>
+      forallb wf es
+  | Mfield (idx, b) =>
+      wf b
+  | Mlazy e => 
+    wf e
+  | Mforce e => wf e
+  | _ => true
+  end
+with wfb (b : binding) : bool :=
+  match b with
+  | Unnamed e => wf e
+  | Named (_, e) => wf e
+  | Recursive l => forallb (fun '(x,e) => wf e) l
+  end.
+
+Fixpoint sapp {A} (l : list A) (env : nat -> A) : nat -> A :=
+  match l with
+  | [] => env
+  | x :: l => sapp l (scons x env)
+  end.
+
+Fixpoint named (env : list string) (x : t) {struct x} : N.t :=
+    match x with
+    | Mvar v => 
+       N.Mvar (nth v env EmptyString)
+    | Mlambda (xs, e) =>
+       N.Mlambda (xs, named (app (rev xs) env) e)
+    | Mapply (f, vs) =>
+        N.Mapply (named env f, map (named env) vs)
+    | Mlet (bindings, body) =>
+        N.Mlet (snd (fold_left (fun '(env, bindings) b => 
+                                    let '(env', b') := namedb env b in
+                                    (env', bindings ++ [b'] )) bindings (env, [])), 
+                                    
+                                named (rev (flat_map bound_names bindings) ++ env) body)
+    | Mnum c => N.Mnum c
+    | Mstring s => N.Mstring s 
+    | Mglobal s => N.Mglobal s
+    | Mswitch (scr, cases) =>
+        N.Mswitch (named env scr, map (fun '(x, e) => (x, named env e)) cases)
+    | Mnumop1 (op, ty, e) =>
+        N.Mnumop1 (op, ty, named env e)
+    | Mnumop2 (op, ty, e1, e2) =>
+        N.Mnumop2 (op, ty, named env e1, named env e2)
+    | Mconvert (ty1, ty2, e) =>
+        N.Mconvert (ty1, ty2, named env e)
+    | Mvecnew (ty, len, def) =>
+        N.Mvecnew(ty, named env len, named env def)
+    | Mvecget (ty, vec, idx) =>
+        N.Mvecget (ty, named env vec, named env idx)
+    | Mvecset (ty, vec, idx, e) => 
+        N.Mvecset (ty, named env vec, named env idx, named env e)
+    | Mveclen (ty, vec) =>
+        N.Mveclen (ty, named env vec)
+    | Mblock (idx, es) => 
+        N.Mblock (idx, map (named env) es)
+    | Mfield (idx, b) =>
+        N.Mfield (idx, named env b)
+    | Mlazy e => N.Mlazy (named env e)
+    | Mforce e => N.Mforce (named env e)
+    end
+with namedb env (b : binding) : list string * N.binding :=
+    match b with
+    | Unnamed e => (env, N.Unnamed (named env e))
+    | Named (x, e) => (x :: env, N.Named (x, named env e))
+    | Recursive l => let nas := map fst l in 
+      (app (rev nas) env, N.Recursive (map (fun '(x,e) => (x, named (app (rev nas) env) e)) l))
+    end.
+    
+Compute (named []
+(Mlambda (["z"%string; "x"%string], Mvar 0))).
+
+Local Open Scope string_scope.
+
+Compute (named []
+  (Mlet
+    ([ Named ("x1", (Mlambda (["z"],Mvar 0))) ;
+       Named ("x2", Mvar 0)
+     ],
+    (Mvar 0))
+)).
+
+(* 
+Goal prod (prod Ident.t (forall _ : nat, Spec.value)) N.t = prod (prod Malfunction.Ident.t (@Malfunction.Ident.Map.t Spec.value))
+    Malfunction.t.
+Proof. cbv. *)
+
+Axiom lookup : Ident.t -> list (Ident.t * value) -> option value.
+
+#[bypass_check(guard)]
+Fixpoint namedv (v : value) : Spec.value :=
+  match v with
+  | Block (idx, vs) => Spec.Block (idx, map namedv vs)
+  | Vec (ty, vs) => Spec.Vec (ty, map (namedv) vs)
+  | Func (x, locals, e) => Spec.Func (x, 
+                                      fun id =>  
+                                         match lookup id locals with 
+                                         | Some v => namedv v 
+                                         | _ => Spec.fail "notfound" 
+                                         end,
+                                      named (cons x (map fst locals)) e)
+  | value_Int x => Spec.value_Int x
+  | Float f => Spec.Float f
+  | Thunk v => Spec.Thunk (namedv v)
+  | fail s => Spec.fail s
+  end.
+
+
+Fixpoint wfv (v : value) : bool :=
+  match v with
+  | Block (idx, vs) => forallb wfv vs
+  | Vec (ty, vs) => forallb wfv vs
+  | Func (x, locals, e) => disj [x] (names e) && wf e
+  | _ => true
+  end.
+
+Definition namede locals : @Ident.Map.t Spec.value :=
+  fun id =>
+  match lookup id locals with 
+  | Some v => namedv v 
+  | _ => Spec.fail "notfound" 
+  end.
+
+Lemma eval_ext l l' e e' v v' :
+  l' = l -> e' = e -> v' = v ->
+  Spec.eval l e v -> Spec.eval l' e' v'.
 Proof.
-  unfold int_of_nat, int_to_nat.
-  rewrite Z2Nat.id.
-  1:eapply Int63.to_Z_bounded.
-  now rewrite Int63.of_to_Z.
+  intros. subst. eauto.
 Qed.
 
-Lemma int_to_of_nat i :
-  (Z.of_nat i < Int63.wB)%Z ->
-  int_to_nat (int_of_nat i) = i.
+Lemma eval_correct locals e v :
+  Forall (fun '(x,v) => wfv v = true) locals ->
+  wf e = true ->
+  eval locals e v ->
+  Spec.eval (namede locals) (named (map fst locals) e) (namedv v).
 Proof.
-  unfold int_of_nat, int_to_nat.
-  intros H.
-  rewrite Int63.of_Z_spec.
-  rewrite Z.mod_small. 1:lia.
-  now rewrite Nat2Z.id.
-Qed.
-
-Lemma Array_of_list'_get {A} s l (a : array A) i :
-  i < s + List.length l ->
-  (s + List.length l < Z.to_nat Int63.wB) ->
-  s + List.length l <= int_to_nat (PArray.length a) ->
-  PArray.get (Array_of_List' s l a) (int_of_nat i) =
-    if (i <? s)%nat then
-      a.[int_of_nat i]
-    else
-      nth (i - s) l (a.[int_of_nat i]).
-Proof.
-  intros Hl Hs Ha.
-  induction l as [ | ? ? IHl] in s, i, a, Hl, Hs, Ha |- *.
-  - destruct (Nat.ltb_spec i s).
-    + cbn. reflexivity.
-    + cbn. destruct (i - s); reflexivity.
-  - rewrite IHl. 
-    + cbn in Hl. lia.
-    + cbn [Datatypes.length] in Hs. lia.
-    + rewrite PArray.length_set. cbn [Datatypes.length] in Ha. lia.
-    + fold (int_of_nat s). destruct (Nat.ltb_spec i s) as [H | H].
-      * destruct (Nat.ltb_spec i (S s)) as [H0 | H0]; try lia.
-        rewrite get_set_other.
-        -- intros E. eapply (f_equal int_to_nat) in E.
-           rewrite !int_to_of_nat in E.
-           all:assert (H1 : s < Z.to_nat Int63.wB) by lia.
-           all:eapply inj_lt in H1.
-           all:rewrite Z2Nat.id in H1. all:lia. 
-        -- reflexivity.
-      * destruct (Nat.ltb_spec i (S s)); try lia.
-        -- assert (i = s) by lia. subst.
-           rewrite get_set_same.
-           ++ eapply Int63.ltb_spec.
-              1:eapply Z2Nat.inj_lt.
-              1:eapply Int63.to_Z_bounded.
-              1:eapply Int63.to_Z_bounded.
-              fold (int_to_nat (int_of_nat s)).
-              rewrite int_to_of_nat. 1:lia.
-              unfold int_to_nat in Ha. lia.
-           ++ cbn. destruct s. 1:reflexivity.
-              rewrite minus_diag. reflexivity.
-        -- cbn. destruct (i - s) as [ | n] eqn:E.
-           ++ lia.
-           ++ assert (H1 : i - S s = n) by lia. rewrite H1.
-              eapply nth_indep.
-              cbn in Hl. lia.
-Qed.
-
-Lemma Array_of_list_get {A} (a : A) l i :
-  (i < Z.to_nat Int63.wB) ->
-  (List.length l < Z.to_nat Int63.wB) ->
-  List.length l <= int_to_nat max_length ->
-  i < List.length l ->
-  PArray.get (Array_of_list a l) (int_of_nat i) = nth i l a.
-Proof.
-  unfold Array_of_list. intros Hs Hl1 Hl Hi.
-  rewrite Array_of_list'_get.
-  + assumption.
-  + lia. 
-  + rewrite PArray.length_make.
-    fold (int_of_nat (Datatypes.length l)).
-    destruct (Int63.lebP (int_of_nat (Datatypes.length l)) max_length) as [ | n ].
-    * rewrite int_to_of_nat.
-      1:eapply Z2Nat.inj_lt. all: lia. 
-    * destruct n.
-      epose proof (int_to_of_nat (Datatypes.length l) _) as H.
-      eapply Z2Nat.inj_le.
-      1:eapply Int63.to_Z_bounded.
-      1:eapply Int63.to_Z_bounded.
-      unfold int_to_nat in H. rewrite H.
-      unfold int_to_nat in Hl. exact Hl.
-      Unshelve. all:lia.
-  + destruct (Nat.ltb_spec i 0); try lia.
-    rewrite Nat.sub_0_r.
-    eapply nth_indep. lia.
-Qed.
-
-Lemma cond_correct scr x :
-  cond scr x = Interpreter.cond (vtrans scr) x.
-Proof. 
-  now destruct x as [ | | [] ], scr as [ [] | [] | [[]] | [] | | | ]. 
-Qed.
-
-Lemma existsb_ext {A} (f g : A -> bool) l :
-  (forall x, f x = g x) ->
-  existsb f l = existsb g l.
-Proof.
-  intros H; induction l; cbn; congruence.
-Qed.
-
-Lemma find_match_correct scr cases e ilocals :
-  find_match scr cases = Some e ->
-  Interpreter.find_match ilocals (vtrans scr) cases = interpret ilocals e.
-Proof.
-  induction cases as [ | a cases IHcases ]; cbn [find_match]; intros Eq.
-  - inversion Eq.
-  - destruct a.
-    + cbn [Interpreter.find_match].
-      destruct existsb eqn:E.
-      * inversion Eq. subst.
-        erewrite existsb_ext.
-        2:{ intros. symmetry. eapply cond_correct. }
-        now rewrite E.
-      * erewrite existsb_ext.
-        2:{ intros. symmetry. eapply cond_correct. }
-        rewrite E. eauto.
-Qed.
-
-Lemma Array_of_list_get_again {A : Set} i s (l : list A) a :
-  i >= s + List.length l ->
-  s + List.length l < Z.to_nat Int63.wB ->
-  i < Z.to_nat Int63.wB ->
-  (Array_of_List' s l a).[int_of_nat i]  = PArray.get a (int_of_nat i).
-Proof.
-  induction l as [ | ? l IHl ] in s, i, a |- *; intros Hi Hs Ha.
-  - cbn. reflexivity.
-  - cbn. rewrite IHl. 
-    + cbn in Hi. lia.
-    + cbn [List.length] in Hs. lia. 
-    + cbn [List.length] in Hs. lia.
-    + rewrite get_set_other. 2:reflexivity.
-      fold (int_of_nat s).
-      intros H. eapply (f_equal int_to_nat) in H.
-      rewrite !int_to_of_nat in H.
-      * eapply inj_lt in Hs.
-        rewrite Z2Nat.id in Hs. 1:cbn; lia.
-        rewrite <- Hs.
-        eapply inj_lt. cbn. lia.
-      * eapply inj_lt in Ha.
-        rewrite Z2Nat.id in Ha. 1:cbn; lia.
-        lia.
-      * subst. cbn in Hi. lia.
-Qed.
-
-Lemma Forall2_map {A B C} (f : A -> B) (g : C -> B) l1 l2 P :
-  Forall2 P l1 l2 ->
-  (forall x y, P x y -> f x = g y) ->
-  map f l1 = map g l2.
-Proof.
-  induction 1; cbn; intros He; f_equal; eauto.
-Qed.
-
-Lemma Func_ext e1 e2 : (forall v, e1 v = e2 v) -> Interpreter.Func e1 = Interpreter.Func e2.
-Proof.
-  intros H. eapply funext in H.
-  subst. reflexivity.
-Qed.
-
-Axiom todo : forall {A : Type}, A.
-
-Lemma eval_correct locals e v ilocals :
-  (forall x, ilocals x = vtrans (locals x)) ->
-  eval locals e v -> interpret ilocals e = vtrans v.
-Proof.
-  intros Hloc.
-  induction 1 as [ (* lambda_sing *) locals x e
-                 | (* lambda *) locals x ids e H
-                 | (* app_sing *) locals x locals' e e2 v2 e1 v H IHeval1 H0 IHeval2 H1 IHeval3
-                 | (* app *) locals idx b vals tag H IHeval 
-                 | (* var *) 
-                 | (* let_body *) | (* let_unnamed *) | (* let_named *) | (* let_rec *)
-                 | (* switch *) loc2 ? ? ? ? ? ? IHeval1 H0 ? IHeval2
-                 | (* block *) loc3 IHeval2 
-                 | (* field *) locals idx b vals tag H IHeval ] 
-    in ilocals, Hloc |- *.
-  1-6,11,12: cbn.
-  11, 12: cycle 1.
-  - eapply Func_ext. intros.
-    f_equal. unfold Ident.Map.add. eapply funext. intros y.
-    unfold Ident.eqb. destruct (String.eqb_spec y x).
+  intros Hloc Hwf Heval.
+  induction Heval; cbn in Hwf.
+  all: repeat match goal with [ H : (_ && _)%bool = true |- _ ] => 
+     let Hwf1 := fresh "Hwf" in
+     let Hwf2 := fresh "Hwf" in
+     eapply Bool.andb_true_iff in H as [Hwf1 Hwf2] end.
+  - cbn. econstructor.
+  - cbn. eapply eval_ext, Spec.eval_lambda; eauto.
+    now rewrite -app_assoc.
+  - cbn. econstructor; eauto.
+    fold namedv (namede locals').
+    eapply eval_ext, IHHeval3; eauto.
+    all: admit.
+  - cbn. econstructor. eapply IHHeval; eauto.
+    cbn. repeat rewrite Bool.andb_true_iff; firstorder.
+  - cbn. eapply eval_ext, Spec.eval_var; eauto.
+    erewrite nth_error_nth.
+    2: now rewrite nth_error_map H.
+    cbn. unfold namede.
+    unfold Malfunction.Ident.Map.find.
+    admit.
+  - cbn. econstructor. eapply IHHeval; eauto.
+  - cbn. eapply eval_ext, Spec.eval_let_unnamed; eauto.
+    + repeat f_equal. admit.
+    + eapply IHHeval2; eauto. cbn.
+      rewrite !Bool.andb_true_iff; firstorder.
+  - cbn. eapply eval_ext, Spec.eval_let_named; eauto.
+    + repeat f_equal. admit.
+    + eapply eval_ext, IHHeval2; eauto. 
+      * admit.
+      * cbn. do 3 f_equal.
+        now rewrite <- !app_assoc.
+      * econstructor; eauto. admit.
+      * cbn. rewrite !Bool.andb_true_iff; firstorder.
+  - cbn. eapply eval_ext, Spec.eval_let_rec; eauto.
+    + repeat f_equal. admit.
+    + admit.
+    + eapply eval_ext, IHHeval; eauto.
+      * cbn. do 3 f_equal.
+        rewrite rev_app_distr -app_assoc. f_equal.
+        admit.
+      * admit.
+      * cbn. rewrite !Bool.andb_true_iff; firstorder.
+        admit.
+  - cbn. econstructor; eauto.
+    + admit.
+    + eapply IHHeval2; eauto. admit.
+  - cbn. econstructor; eauto.
+    admit.
+  - cbn. eapply eval_ext, Spec.eval_field.
     + reflexivity.
-    + eauto.
-  - destruct ids as [ | t ids ]; cbn in H. 1:inversion H. clear H.
-      cbn. eapply Func_ext. intros ?.
-      destruct match ids with
-               | [] => (t, e)
-               | _ :: _ => (t, Mlambda (ids, e))
-               end eqn:E.
-      rewrite E.
-      eapply Func_ext. intros.
-      repeat f_equal. 
-      eapply funext. eauto. 
-  - rewrite IHeval1; [eauto |].
-    cbn. cbn in IHeval3.
-    erewrite <- IHeval3 with (ilocals := fun x0 => vtrans (Ident.Map.add x v2 locals' x0)).
-    2: reflexivity.
-    f_equal.
-    eapply funext. 
-    intros x0. unfold Ident.Map.add.
-    unfold Ident.eqb. destruct (String.eqb_spec x0 x).
-    + eapply IHeval2. eauto.
     + reflexivity.
-  - cbn in IHeval. eauto.
-  - unfold Ident.Map.find. eauto.
-  - eauto.
-  - repeat f_equal. eapply Forall2_map.
-    1:eassumption.
-    intros. cbn in *. eauto.
-  -  rewrite IHeval. 1:eauto.
-    cbn. rewrite <- (int_of_to_nat idx).
-    assert (int_to_nat idx < List.length vals \/ int_to_nat idx >= List.length vals)  as [Hl | Hl] by lia.
-    + rewrite Array_of_list_get.
-      * eapply Z2Nat.inj_lt.
-        1:eapply Int63.to_Z_bounded; cbn. 1: lia.
-        1:eapply Int63.to_Z_bounded.
-      * rewrite map_length. assumption.
-      * rewrite map_length. assumption.
-      * now rewrite map_length.
-      * change (Interpreter.fail "") with (vtrans (fail "")).
-        rewrite int_of_to_nat.
-        eapply map_nth.
-    + rewrite nth_overflow.
-      * rewrite int_to_of_nat. 1:unfold int_to_nat.
-        1:rewrite Z2Nat.id. 1:eapply Int63.to_Z_bounded.
-        1:eapply Int63.to_Z_bounded. lia.
-      * unfold Array_of_list. rewrite Array_of_list_get_again.
-        -- rewrite map_length. lia.
-        -- rewrite map_length. cbn [plus]. assumption.
-        -- unfold int_to_nat. eapply Z2Nat.inj_lt.
-           1:eapply Int63.to_Z_bounded.
-           1: cbn. 1: lia. 1:eapply Int63.to_Z_bounded.
-        -- rewrite get_make. reflexivity.
-  - cbn. eapply IHeval2. eauto.
-  - cbn. eapply IHeval2. intros.
-    rewrite IHeval1. 1:eauto.
-    unfold Ident.Map.add, Ident.eqb.
-    destruct (String.eqb_spec x0 x); eauto.
-  - cbn [interpret].
-    erewrite <- IHeval2; eauto.
-    eapply find_match_correct in H0.
-    rewrite <- H0.
-    rewrite IHeval1; eauto.
-Guarded. 
-Unset Guard Checking.
-  - cbn.  eapply IHeval. intros x.
-    clear - H Hloc. revert H.
-    unfold add_recs.
-    rewrite newlocals_eqn.
-    generalize recs at 1 3.
-    intros allrecs H.
-    induction recs as [ | (f, e) recs IH] in allrecs, ilocals, locals, H, newlocals, Hloc |- *.
-    + cbn in H |- *. inversion H as [E]; subst. eapply Hloc.
-    + cbn in H |- *. destruct e; try now inversion H.
-      destruct p as (bindings, e).
-      destruct bindings as [ | y ]; try now inversion H.
-      destruct add_recs' as [ newlocals' | ] eqn:E; inversion H. subst. clear H. 
-      unfold Ident.Map.add, Ident.eqb.
-      destruct (String.eqb_spec x f).
-      2: eapply IH; eauto.
-      subst. cbn. clear IH.
-      eapply Func_ext. intros v.
-      enough (interpret
-      (Ident.Map.add y v
-         (fun x : Ident.t => newlocals interpret allrecs ilocals x))
-      (Mklambda bindings e) = interpret
-      (newlocals interpret allrecs
-         (Ident.Map.add y v (fun x : Ident.t => vtrans (newlocals' x))))
-      (Mklambda (bindings) e)) by (destruct bindings; eauto).
-      f_equal. eapply funext in Hloc. subst. 
-      (* This is true: y is not in allrecs.
-          lemma 1: adding recs to locals and looking up an ident not in recs is equivalent to locals
-          lemma 2: newlocals yields the same environment if passed locals1 and locals2 which are equal _outside of_ recs      
-      *)
-      apply todo.
-Qed.
-Set Guard Checking.
+    + admit.
+    + eapply IHHeval; eauto.
+    + admit.
+    + admit.
+Admitted.
