theories/SemanticsSpec.v
@@ -1,0 +1,484 @@
+Require Import ssreflect.
+From Malfunction Require Import Malfunction Interpreter.
+
+Require Import ZArith Array.PArray List String Floats Lia.
+Import ListNotations.
+
+Set Default Goal Selector "!".
+
+Inductive value :=
+| Block of int * list value
+| Vec of vector_type * list value
+| Func of Ident.t * @Ident.Map.t value * t
+| value_Int of inttype * Z
+| Float of float
+| Thunk of value
+| fail of string
+.
+
+Fixpoint vtrans (s : value) : Interpreter.value :=
+  match s with
+  | Block (tag, vals) => Interpreter.Block (tag, Array_of_list (Interpreter.fail "") (map vtrans vals))
+  | Vec (ty, vals) => Interpreter.Vec (ty, Array_of_list (Interpreter.fail "") (map vtrans vals))
+  | Func (x, locals, e) => Interpreter.Func (fun v => interpret (Ident.Map.add x v (fun x => vtrans (locals x))) e)
+  | value_Int (ty, i) => Interpreter.value_Int (ty, i)
+  | Float f => Interpreter.Float f
+  | Thunk v => Interpreter.Thunk (vtrans v)
+  | fail x => Interpreter.fail x
+  end.
+
+Definition int_to_nat (i : int) : nat :=
+  Z.to_nat (Int63.to_Z i).
+
+
+Definition cond scr case : bool := 
+  (match case, scr with
+    | Tag n, Block (n', _) => Int63.eqb n n'
+    | Deftag, Block _ => true
+    | Intrange (min, max), value_Int (Int, n) => Z.leb (Int63.to_Z min) n && Z.leb n (Int63.to_Z max)
+    | _, _ => false end).
+
+Fixpoint find_match scr x : option t := match x with 
+                                        | (cases, e) :: rest =>
+                                            if List.existsb (cond scr) cases then
+                                              Some e
+                                            else
+                                              find_match scr rest
+                                        | [] => None end.
+
+
+Definition Mklambda binders e :=
+  match binders with [] => e | _ => Mlambda (binders, e) end.
+
+Fixpoint add_recs' (locals : Ident.Map.t) allrecs recs  :=
+  match recs with
+  | [] => Some locals
+  | (x, Mlambda (y :: more, e)) :: recs =>  
+    match add_recs' locals allrecs recs with
+    | Some locals => Some (Ident.Map.add x (Func (y, locals, Mlet ([Recursive allrecs], Mklambda more e))) locals)
+    | None => None
+    end
+  | _ => None
+  end.
+Definition add_recs locals recs := add_recs' locals recs recs.
+
+Unset Elimination Schemes.           
+Inductive eval (locals : @Ident.Map.t value) : t -> value -> Prop :=
+| eval_lambda_sing x e :
+  eval locals (Mlambda ([x], e)) (Func (x, locals, e))
+| eval_lambda x ids e :
+  List.length ids > 0 ->
+  eval locals (Mlambda (x :: ids, e)) (Func (x, locals, Mlambda (ids, e)))
+| eval_app_sing x locals' e e2 v2 e1 v :
+  eval locals e1 (Func (x, locals', e)) -> eval locals e2 v2 ->
+  eval (Ident.Map.add x v2 locals') e v ->
+  eval locals (Mapply (e1, [e2])) v
+| eval_app e2 e1 v es :
+  eval locals (Mapply (Mapply (e1, [e2]), es)) v ->
+  eval locals (Mapply (e1, e2 :: es)) v
+| eval_var id :
+  eval locals (Mvar id) (Ident.Map.find id locals)
+| eval_let_body e v : 
+  eval locals e v -> eval locals (Mlet ([], e)) v
+| eval_let_unnamed e1 v1 lts e2 v :
+  eval locals e1 v1 ->
+  eval locals (Mlet (lts, e2)) v ->
+  eval locals (Mlet (Unnamed e1 :: lts, e2)) v 
+| eval_let_named x e1 v1 lts e2 v :
+  eval locals e1 v1 ->
+  eval (Ident.Map.add x v1 locals) (Mlet (lts, e2)) v ->
+  eval locals (Mlet (Named (x,e1) :: lts, e2)) v 
+| eval_let_rec recs newlocals lts e2 v :
+  add_recs locals recs = Some newlocals ->
+  eval newlocals (Mlet (lts, e2)) v ->
+  eval locals (Mlet (Recursive recs :: lts, e2)) v 
+| eval_switch scr cases v v' e :
+  eval locals scr v' ->
+  find_match v' cases = Some e ->
+  eval locals e v ->
+  eval locals (Mswitch (scr, cases)) v
+| eval_block tag es vals :
+  Forall2 (eval locals) es vals ->
+  eval locals (Mblock (tag, es)) (Block (tag, vals))
+| eval_field idx b vals tag :
+  eval locals b (Block (tag, vals)) ->
+  Datatypes.length vals < Z.to_nat Int63.wB ->
+  Datatypes.length vals <= int_to_nat max_length ->
+  eval locals (Mfield (idx, b)) (nth (int_to_nat idx) vals (fail "")).
+
+Lemma eval_ind :
+forall P : Ident.Map.t -> t -> value -> Prop,
+(forall (locals : Ident.Map.t) (x : Ident.t) (e : t),
+ P locals (Mlambda ([x], e)) (Func (x, locals, e))) ->
+(forall (locals : Ident.Map.t) (x : Ident.t) (ids : list Ident.t) (e : t),
+ Datatypes.length ids > 0 ->
+ P locals (Mlambda (x :: ids, e)) (Func (x, locals, Mlambda (ids, e)))) ->
+(forall (locals : Ident.Map.t) (x : Ident.t) (locals' : Ident.Map.t) 
+   (e e2 : t) (v2 : value) (e1 : t) (v : value),
+ eval locals e1 (Func (x, locals', e)) ->
+ P locals e1 (Func (x, locals', e)) ->
+ eval locals e2 v2 ->
+ P locals e2 v2 ->
+ eval (Ident.Map.add x v2 locals') e v ->
+ P (Ident.Map.add x v2 locals') e v -> P locals (Mapply (e1, [e2])) v) ->
+(forall (locals : Ident.Map.t) (e2 e1 : t) (v : value) (es : list t),
+ eval locals (Mapply (Mapply (e1, [e2]), es)) v ->
+ P locals (Mapply (Mapply (e1, [e2]), es)) v -> P locals (Mapply (e1, e2 :: es)) v) ->
+(forall (locals : Ident.Map.t) (id : Ident.t),
+ P locals (Mvar id) (Ident.Map.find id locals)) ->
+ (forall (locals : Ident.Map.t) (e : t) (v : value),
+ eval locals e v -> P locals e v -> P locals (Mlet ([], e)) v) ->
+(forall (locals : Ident.Map.t) (e1 : t) (v1 : value) 
+   (lts : list binding) (e2 : t) (v : value),
+ eval locals e1 v1 ->
+ P locals e1 v1 ->
+ eval locals (Mlet (lts, e2)) v ->
+ P locals (Mlet (lts, e2)) v -> P locals (Mlet (Unnamed e1 :: lts, e2)) v) ->
+(forall (locals : Ident.Map.t) (x : Ident.t) (e1 : t) 
+   (v1 : value) (lts : list binding) (e2 : t) (v : value),
+ eval locals e1 v1 ->
+ P locals e1 v1 ->
+ eval (Ident.Map.add x v1 locals) (Mlet (lts, e2)) v ->
+ P (Ident.Map.add x v1 locals) (Mlet (lts, e2)) v ->
+ P locals (Mlet (Named (x, e1) :: lts, e2)) v) ->
+(forall (locals : Ident.Map.t) (recs : list (Ident.t * t))
+   (newlocals : Ident.Map.t) (lts : list binding) 
+   (e2 : t) (v : value),
+ add_recs locals recs = Some newlocals ->
+ eval newlocals (Mlet (lts, e2)) v ->
+ P newlocals (Mlet (lts, e2)) v ->
+ P locals (Mlet (Recursive recs :: lts, e2)) v) ->
+(forall (locals : Ident.Map.t) (scr : t) (cases : list (list case * t))
+   (v v' : value) (e : t),
+ eval locals scr v' ->
+ P locals scr v' ->
+ find_match v' cases = Some e ->
+ eval locals e v -> P locals e v -> P locals (Mswitch (scr, cases)) v) ->
+(forall (locals : Ident.Map.t) (tag : int) (es : list t) (vals : list value),
+    Forall2 (eval locals) es vals ->
+    Forall2 (P locals) es vals ->
+    P locals (Mblock (tag, es)) (Block (tag, vals))) ->
+(forall (locals : Ident.Map.t) (idx : int) (b : t) (vals : list value) (tag : int),
+ eval locals b (Block (tag, vals)) ->
+ P locals b (Block (tag, vals)) ->
+ Datatypes.length vals < Z.to_nat Int63.wB ->
+ Datatypes.length vals <= int_to_nat max_length ->
+ P locals (Mfield (idx, b)) (nth (int_to_nat idx) vals (fail ""))) ->
+forall (locals : Ident.Map.t) (t : t) (v : value), eval locals t v -> P locals t v.
+Proof.
+  intros P H_lambda_sing H_lambda H_app_sing H_app H_var H_let_body H_let_unnamed H_let_named 
+        H_let_rec H_switch H_block H_field.
+  fix f 4. intros locals t v [ | | | | | | | | | | ? ? ? Hforall | ].
+  1-10: eauto.
+  - eapply H_block. 1: eauto. induction Hforall. 
+    + econstructor.  
+    + econstructor; eauto.
+  - eapply H_field. 1: eauto. 1: eauto. all: lia.
+Qed.
+Set Elimination Schemes.
+
+Axiom funext : forall A B, forall f g : A -> B, (forall x, f x = g x) -> f = g.
+
+Definition int_of_nat n := Int63.of_Z (Z.of_nat n).
+
+Lemma int_of_to_nat i :
+  int_of_nat (int_to_nat i) = i.
+Proof.
+  unfold int_of_nat, int_to_nat.
+  rewrite Z2Nat.id.
+  1:eapply Int63.to_Z_bounded.
+  now rewrite Int63.of_to_Z.
+Qed.
+
+Lemma int_to_of_nat i :
+  (Z.of_nat i < Int63.wB)%Z ->
+  int_to_nat (int_of_nat i) = i.
+Proof.
+  unfold int_of_nat, int_to_nat.
+  intros H.
+  rewrite Int63.of_Z_spec.
+  rewrite Z.mod_small. 1:lia.
+  now rewrite Nat2Z.id.
+Qed.
+
+Lemma Array_of_list'_get {A} s l (a : array A) i :
+  i < s + List.length l ->
+  (s + List.length l < Z.to_nat Int63.wB) ->
+  s + List.length l <= int_to_nat (PArray.length a) ->
+  PArray.get (Array_of_List' s l a) (int_of_nat i) =
+    if (i <? s)%nat then
+      a.[int_of_nat i]
+    else
+      nth (i - s) l (a.[int_of_nat i]).
+Proof.
+  intros Hl Hs Ha.
+  induction l as [ | ? ? IHl] in s, i, a, Hl, Hs, Ha |- *.
+  - destruct (Nat.ltb_spec i s).
+    + cbn. reflexivity.
+    + cbn. destruct (i - s); reflexivity.
+  - rewrite IHl. 
+    + cbn in Hl. lia.
+    + cbn [Datatypes.length] in Hs. lia.
+    + rewrite PArray.length_set. cbn [Datatypes.length] in Ha. lia.
+    + fold (int_of_nat s). destruct (Nat.ltb_spec i s) as [H | H].
+      * destruct (Nat.ltb_spec i (S s)) as [H0 | H0]; try lia.
+        rewrite get_set_other.
+        -- intros E. eapply (f_equal int_to_nat) in E.
+           rewrite !int_to_of_nat in E.
+           all:assert (H1 : s < Z.to_nat Int63.wB) by lia.
+           all:eapply inj_lt in H1.
+           all:rewrite Z2Nat.id in H1. all:lia. 
+        -- reflexivity.
+      * destruct (Nat.ltb_spec i (S s)); try lia.
+        -- assert (i = s) by lia. subst.
+           rewrite get_set_same.
+           ++ eapply Int63.ltb_spec.
+              1:eapply Z2Nat.inj_lt.
+              1:eapply Int63.to_Z_bounded.
+              1:eapply Int63.to_Z_bounded.
+              fold (int_to_nat (int_of_nat s)).
+              rewrite int_to_of_nat. 1:lia.
+              unfold int_to_nat in Ha. lia.
+           ++ cbn. destruct s. 1:reflexivity.
+              rewrite minus_diag. reflexivity.
+        -- cbn. destruct (i - s) as [ | n] eqn:E.
+           ++ lia.
+           ++ assert (H1 : i - S s = n) by lia. rewrite H1.
+              eapply nth_indep.
+              cbn in Hl. lia.
+Qed.
+
+Lemma Array_of_list_get {A} (a : A) l i :
+  (i < Z.to_nat Int63.wB) ->
+  (List.length l < Z.to_nat Int63.wB) ->
+  List.length l <= int_to_nat max_length ->
+  i < List.length l ->
+  PArray.get (Array_of_list a l) (int_of_nat i) = nth i l a.
+Proof.
+  unfold Array_of_list. intros Hs Hl1 Hl Hi.
+  rewrite Array_of_list'_get.
+  + assumption.
+  + lia. 
+  + rewrite PArray.length_make.
+    fold (int_of_nat (Datatypes.length l)).
+    destruct (Int63.lebP (int_of_nat (Datatypes.length l)) max_length) as [ | n ].
+    * rewrite int_to_of_nat.
+      1:eapply Z2Nat.inj_lt. all: lia. 
+    * destruct n.
+      epose proof (int_to_of_nat (Datatypes.length l) _) as H.
+      eapply Z2Nat.inj_le.
+      1:eapply Int63.to_Z_bounded.
+      1:eapply Int63.to_Z_bounded.
+      unfold int_to_nat in H. rewrite H.
+      unfold int_to_nat in Hl. exact Hl.
+      Unshelve. all:lia.
+  + destruct (Nat.ltb_spec i 0); try lia.
+    rewrite Nat.sub_0_r.
+    eapply nth_indep. lia.
+Qed.
+
+Lemma cond_correct scr x :
+  cond scr x = Interpreter.cond (vtrans scr) x.
+Proof. 
+  now destruct x as [ | | [] ], scr as [ [] | [] | [[]] | [] | | | ]. 
+Qed.
+
+Lemma existsb_ext {A} (f g : A -> bool) l :
+  (forall x, f x = g x) ->
+  existsb f l = existsb g l.
+Proof.
+  intros H; induction l; cbn; congruence.
+Qed.
+
+Lemma find_match_correct scr cases e ilocals :
+  find_match scr cases = Some e ->
+  Interpreter.find_match ilocals (vtrans scr) cases = interpret ilocals e.
+Proof.
+  induction cases as [ | a cases IHcases ]; cbn [find_match]; intros Eq.
+  - inversion Eq.
+  - destruct a.
+    + cbn [Interpreter.find_match].
+      destruct existsb eqn:E.
+      * inversion Eq. subst.
+        erewrite existsb_ext.
+        2:{ intros. symmetry. eapply cond_correct. }
+        now rewrite E.
+      * erewrite existsb_ext.
+        2:{ intros. symmetry. eapply cond_correct. }
+        rewrite E. eauto.
+Qed.
+
+Lemma Array_of_list_get_again {A : Set} i s (l : list A) a :
+  i >= s + List.length l ->
+  s + List.length l < Z.to_nat Int63.wB ->
+  i < Z.to_nat Int63.wB ->
+  (Array_of_List' s l a).[int_of_nat i]  = PArray.get a (int_of_nat i).
+Proof.
+  induction l as [ | ? l IHl ] in s, i, a |- *; intros Hi Hs Ha.
+  - cbn. reflexivity.
+  - cbn. rewrite IHl. 
+    + cbn in Hi. lia.
+    + cbn [List.length] in Hs. lia. 
+    + cbn [List.length] in Hs. lia.
+    + rewrite get_set_other. 2:reflexivity.
+      fold (int_of_nat s).
+      intros H. eapply (f_equal int_to_nat) in H.
+      rewrite !int_to_of_nat in H.
+      * eapply inj_lt in Hs.
+        rewrite Z2Nat.id in Hs. 1:cbn; lia.
+        rewrite <- Hs.
+        eapply inj_lt. cbn. lia.
+      * eapply inj_lt in Ha.
+        rewrite Z2Nat.id in Ha. 1:cbn; lia.
+        lia.
+      * subst. cbn in Hi. lia.
+Qed.
+
+Lemma Forall2_map {A B C} (f : A -> B) (g : C -> B) l1 l2 P :
+  Forall2 P l1 l2 ->
+  (forall x y, P x y -> f x = g y) ->
+  map f l1 = map g l2.
+Proof.
+  induction 1; cbn; intros He; f_equal; eauto.
+Qed.
+
+Lemma Func_ext e1 e2 : (forall v, e1 v = e2 v) -> Interpreter.Func e1 = Interpreter.Func e2.
+Proof.
+  intros H. eapply funext in H.
+  subst. reflexivity.
+Qed.
+
+Axiom todo : forall {A : Type}, A.
+
+(* Lemma newlocals_env interpret recs locals1 locals2 x :
+  (forall x, ~ In x (map fst recs) -> locals1 x = locals2 x) ->
+  newlocals interpret recs locals1 x =
+  newlocals interpret recs locals2 x.
+Proof.
+  rewrite !newlocals_eqn.
+  generalize recs at 2 4.
+  intros allrecs Hext.
+  induction recs as [ | [] ].
+  - cbn. eapply Hext. firstorder.
+  - cbn. f_equal.
+    + destruct t0; try reflexivity.
+      eapply Func_ext. *)
+
+Lemma eval_correct locals e v ilocals :
+  (forall x, ilocals x = vtrans (locals x)) ->
+  eval locals e v -> interpret ilocals e = vtrans v.
+Proof.
+  intros Hloc.
+  induction 1 as [ (* lambda_sing *) locals x e
+                 | (* lambda *) locals x ids e H
+                 | (* app_sing *) locals x locals' e e2 v2 e1 v H IHeval1 H0 IHeval2 H1 IHeval3
+                 | (* app *) locals idx b vals tag H IHeval 
+                 | (* var *) 
+                 | (* let_body *) | (* let_unnamed *) | (* let_named *) | (* let_rec *)
+                 | (* switch *) loc2 ? ? ? ? ? ? IHeval1 H0 ? IHeval2
+                 | (* block *) loc3 IHeval2 
+                 | (* field *) locals idx b vals tag H IHeval ] 
+    in ilocals, Hloc |- *.
+  1-6,11,12: cbn.
+  11, 12: cycle 1.
+  - eapply Func_ext. intros.
+    f_equal. unfold Ident.Map.add. eapply funext. intros y.
+    unfold Ident.eqb. destruct (String.eqb_spec y x).
+    + reflexivity.
+    + eauto.
+  - destruct ids as [ | t ids ]; cbn in H. 1:inversion H. clear H.
+      cbn. eapply Func_ext. intros ?.
+      destruct match ids with
+               | [] => (t, e)
+               | _ :: _ => (t, Mlambda (ids, e))
+               end eqn:E.
+      rewrite E.
+      eapply Func_ext. intros.
+      repeat f_equal. 
+      eapply funext. eauto. 
+  - rewrite IHeval1; [eauto |].
+    cbn. cbn in IHeval3.
+    erewrite <- IHeval3 with (ilocals := fun x0 => vtrans (Ident.Map.add x v2 locals' x0)).
+    2: reflexivity.
+    f_equal.
+    eapply funext. 
+    intros x0. unfold Ident.Map.add.
+    unfold Ident.eqb. destruct (String.eqb_spec x0 x).
+    + eapply IHeval2. eauto.
+    + reflexivity.
+  - cbn in IHeval. eauto.
+  - unfold Ident.Map.find. eauto.
+  - eauto.
+  - repeat f_equal. eapply Forall2_map.
+    1:eassumption.
+    intros. cbn in *. eauto.
+  -  rewrite IHeval. 1:eauto.
+    cbn. rewrite <- (int_of_to_nat idx).
+    assert (int_to_nat idx < List.length vals \/ int_to_nat idx >= List.length vals)  as [Hl | Hl] by lia.
+    + rewrite Array_of_list_get.
+      * eapply Z2Nat.inj_lt.
+        1:eapply Int63.to_Z_bounded; cbn. 1: lia.
+        1:eapply Int63.to_Z_bounded.
+      * rewrite map_length. assumption.
+      * rewrite map_length. assumption.
+      * now rewrite map_length.
+      * change (Interpreter.fail "") with (vtrans (fail "")).
+        rewrite int_of_to_nat.
+        eapply map_nth.
+    + rewrite nth_overflow.
+      * rewrite int_to_of_nat. 1:unfold int_to_nat.
+        1:rewrite Z2Nat.id. 1:eapply Int63.to_Z_bounded.
+        1:eapply Int63.to_Z_bounded. lia.
+      * unfold Array_of_list. rewrite Array_of_list_get_again.
+        -- rewrite map_length. lia.
+        -- rewrite map_length. cbn [plus]. assumption.
+        -- unfold int_to_nat. eapply Z2Nat.inj_lt.
+           1:eapply Int63.to_Z_bounded.
+           1: cbn. 1: lia. 1:eapply Int63.to_Z_bounded.
+        -- rewrite get_make. reflexivity.
+  - cbn. eapply IHeval2. eauto.
+  - cbn. eapply IHeval2. intros.
+    rewrite IHeval1. 1:eauto.
+    unfold Ident.Map.add, Ident.eqb.
+    destruct (String.eqb_spec x0 x); eauto.
+  - cbn [interpret].
+    erewrite <- IHeval2; eauto.
+    eapply find_match_correct in H0.
+    rewrite <- H0.
+    rewrite IHeval1; eauto.
+Guarded. 
+Unset Guard Checking.
+  - cbn. eapply IHeval. intros x.
+    clear - H Hloc. revert H.
+    unfold add_recs.
+    rewrite newlocals_eqn.
+    generalize recs at 1 3.
+    intros allrecs H.
+    induction recs as [ | (f, e) recs IH] in allrecs, ilocals, locals, H, newlocals, Hloc |- *.
+    + cbn in H |- *. inversion H as [E]; subst. eapply Hloc.
+    + cbn in H |- *. destruct e; try now inversion H.
+      destruct p as (bindings, e).
+      destruct bindings as [ | y ]; try now inversion H.
+      destruct add_recs' as [ newlocals' | ] eqn:E; inversion H. subst. clear H. 
+      unfold Ident.Map.add, Ident.eqb.
+      destruct (String.eqb_spec x f).
+      2: eapply IH; eauto.
+      subst. cbn [vtrans]. clear IH.
+      eapply Func_ext. intros v. unfold interpret at 1. fold interpret.
+      enough (
+        interpret
+        (Ident.Map.add y v
+           (fun x : Ident.t => newlocals interpret allrecs ilocals x))
+        (Mklambda bindings e) =
+      interpret (Ident.Map.add y v (fun x : Ident.t => vtrans (newlocals' x)))
+        (Mlet ([Recursive allrecs], Mklambda bindings e))) by (destruct bindings; eauto).
+      generalize (Mklambda bindings e). clear e. intros e.
+      cbn.
+      f_equal. eapply funext in Hloc. subst. 
+      (* This is true: y is not in allrecs.
+          lemma 1: adding recs to locals and looking up an ident not in recs is equivalent to locals
+          lemma 2: newlocals yields the same environment if passed locals1 and locals2 which are equal _outside of_ recs      
+      *)
+      apply todo.
+Qed.
+Set Guard Checking.
